providers/evercrypt/fst/EverCrypt.Hash.Test.fst
@@ -1,0 +1,99 @@
+module EverCrypt.Hash.Test 
+
+open FStar.HyperStack.ST
+open FStar.Integers  
+open FStar.Seq
+open EverCrypt.Hash
+
+module ST = FStar.HyperStack.ST
+module B = LowStar.Buffer
+module M = LowStar.Modifies
+
+/// As a sanity check, we program & verify the whole hash algorithm
+/// from its low-level incremental API.  We could compare their
+/// extracted code & performance, and similarly provide a shared
+/// reference implementation of update_multi.
+
+[@"c_inline"] // due to variable-length stack allocation
+val compute: 
+  a: alg ->
+  len: UInt32.t -> 
+  text: uint8_pl (v len) -> 
+  tag: uint8_pl (tagLength (Ghost.hide a)) -> ST unit
+  (requires fun h0 -> 
+    B.live h0 text /\ 
+    B.live h0 tag /\ 
+    M.(loc_disjoint (loc_buffer text) (loc_buffer tag)))
+  (ensures fun h0 () h1 -> 
+    B.live h1 text /\ B.live h1 tag /\
+    // M.(modifies (loc_buffer tag) h0 h1) /\
+    v len <= maxLength (Ghost.hide a) /\ (* required for subtyping the RHS below *)
+    B.as_seq h1 tag = spec (Ghost.hide a) (B.as_seq h0 text))
+//18-07-07 TODO add dealloation; restore Stack (not ST); restore modifies clause
+
+#reset-options "--z3rlimit 300"
+let compute a len text tag = 
+  push_frame();
+  let s = create a in 
+  assert_norm(v len <= maxLength (Ghost.hide a));
+  let ll = FStar.UInt32.(len %^ blockLen a) in
+  let lb = FStar.UInt32.(len -^ ll)in
+  let blocks = B.sub text 0ul lb in
+  let last = B.offset text lb in
+  let h1 = ST.get() in 
+  init s; 
+  let h10 = ST.get() in 
+  assert(well_formed s h10);
+  assume(bounded_counter s h10 (v lb));
+  assert(invariant s h10);
+  update_multi s blocks lb; 
+  let h11 = ST.get() in 
+  assert(well_formed s h11);
+  assume(bounded_counter s h11 2);
+  update_last s last len;
+  finish s tag;
+  let h2 = ST.get() in 
+  pop_frame();
+  ( let vblocks = B.as_seq h1 blocks in 
+    let vlast = B.as_seq h1 last in 
+    let vsuffix = suffix (Ghost.hide a) (v len) in
+    Seq.lemma_eq_intro (B.as_seq h1 text) (vblocks @| vlast);
+    lemma_hash2 (acc0 #(Ghost.hide a)) vblocks (vlast @| vsuffix); 
+    Seq.append_assoc vblocks vlast vsuffix )
+
+(*
+val compute: 
+  a: alg13 ->
+  len: UInt32.t -> 
+  text: uint8_pl (v len) -> 
+  tag: uint8_pl (tagLength a){ disjoint text tag } -> Stack unit
+  (requires fun h0 -> 
+    live h0 text /\ live h0 tag)
+  (ensures fun h0 () h1 -> 
+    live h1 text /\ live h1 tag /\
+    modifies_1 tag h0 h1 /\
+    v len <= maxLength a /\ (* required for subtyping the RHS below *)
+    as_seq h1 tag = spec a (as_seq h0 text))
+let compute a len test tag = 
+  match a with 
+  | SHA256 -> hash a len test tag
+  | SHA384 -> hash a len test tag
+  | SHA512 -> hash a len test tag 
+*)
+
+val test: 
+  a: alg13 -> 
+  len: UInt32.t -> 
+  text: uint8_pl (v len) -> ST unit
+  (requires fun h0 -> B.live h0 text)
+  (ensures fun h0 _ h1 -> True //TODO adapt modifies_0 h0 h1
+  )
+
+let test a len data = 
+  push_frame();
+  let tag0 = B.alloca 0uy (tagLen a) in
+  let tag1 = B.alloca 0uy (tagLen a) in
+  assert_norm(pow2 32 <= maxLength (Ghost.hide a));
+  EverCrypt.Hash.hash a tag0 data len;
+  compute a len data tag1;
+  pop_frame()
